cedar-lean/Cedar/Thm/WellTyped.lean
@@ -434,19 +434,194 @@ theorem typechecked_is_well_typed_after_lifting {e : Expr} {c₁ c₂ : Capabili
         apply @TypedExpr.WellTyped.getAttr_record _ (.mk (CedarType.liftBoolTypesRecord rty.1))
         · exact typechecked_is_well_typed_after_lifting h₂ hᵢ
         · simp [type_of_after_lifted_is_lifted, heq, CedarType.liftBoolTypes]
-        · simp only [Option.map_eq_some']
+        · simp
           simp [getAttrInRecord] at h₃₁
-          split at h₃₁
-          case _ heq₁ =>
-            sorry
+          split at h₃₁ <;> try
+          {
+            rename_i aty heq₁
+            simp [ok] at h₃₁
+            rcases h₃₁ with ⟨h₃₁, _⟩
+            exists QualifiedType.liftBoolTypes (.required aty)
+            apply And.intro
+            · simp [lift_bool_types_record_eq_map_on_values,
+                Data.Map.find?_mapOnValues_some QualifiedType.liftBoolTypes heq₁]
+            · subst h₃₁
+              simp [QualifiedType.liftBoolTypes, Qualified.getType]
+          }
           case _ =>
-            sorry
+            split at h₃₁
+            case _ aty heq₁ _ =>
+              simp [ok] at h₃₁
+              rcases h₃₁ with ⟨h₃₁, _⟩
+              exists QualifiedType.liftBoolTypes (.optional aty)
+              apply And.intro
+              · simp [lift_bool_types_record_eq_map_on_values,
+                Data.Map.find?_mapOnValues_some QualifiedType.liftBoolTypes heq₁]
+              · subst h₃₁
+                simp [QualifiedType.liftBoolTypes, Qualified.getType]
+            case _ => simp [err] at h₃₁
           case _ => simp [err] at h₃₁
-      case _ => sorry
+      case _ ety heq =>
+        split at h₃
+        case _ rty heq₁ =>
+          simp [ok, do_ok] at h₃
+          rcases h₃ with ⟨a, h₃₁, h₃₂⟩
+          subst h₃₂
+          simp [TypedExpr.liftBoolTypes]
+          apply @TypedExpr.WellTyped.getAttr_entity _ ety (.mk (CedarType.liftBoolTypesRecord rty.1))
+          · exact typechecked_is_well_typed_after_lifting h₂ hᵢ
+          · simp [type_of_after_lifted_is_lifted, heq, CedarType.liftBoolTypes]
+          · simp [heq₁, RecordType.liftBoolTypes]
+          · simp
+            -- repeat the proofs on record get attr
+            sorry
+        case _ => simp [err] at h₃
       case _ => simp [err] at h₃
-  case hasAttr => sorry
-  case set => sorry
+  case hasAttr x₁ attr =>
+    simp [typeOf] at h₃
+    generalize hᵢ : typeOf x₁ c₁ env = res₁
+    cases res₁
+    case error => simp [hᵢ] at h₃
+    case ok ty =>
+      simp [hᵢ] at h₃
+      simp [typeOfHasAttr] at h₃
+      split at h₃
+      case _ rty heq =>
+        simp [ok, do_ok] at h₃
+        rcases h₃ with ⟨_, h₃₁, h₃₂⟩
+        subst h₃₂
+        simp [TypedExpr.liftBoolTypes]
+        simp [hasAttrInRecord] at h₃₁
+        split at h₃₁
+        · split at h₃₁ <;>
+          {
+            simp [ok] at h₃₁
+            rcases h₃₁ with ⟨h₃₁, _⟩
+            subst h₃₁
+            simp [CedarType.liftBoolTypes, BoolType.lift]
+            apply @TypedExpr.WellTyped.hasAttr_record env (RecordType.liftBoolTypes rty)
+            · exact typechecked_is_well_typed_after_lifting h₂ hᵢ
+            · simp [type_of_after_lifted_is_lifted, heq, CedarType.liftBoolTypes, RecordType.liftBoolTypes]
+          }
+        · simp [ok] at h₃₁
+          rcases h₃₁ with ⟨h₃₁, _⟩
+          subst h₃₁
+          simp [CedarType.liftBoolTypes, BoolType.lift]
+          apply @TypedExpr.WellTyped.hasAttr_record env (RecordType.liftBoolTypes rty)
+          · exact typechecked_is_well_typed_after_lifting h₂ hᵢ
+          · simp [type_of_after_lifted_is_lifted, heq, CedarType.liftBoolTypes, RecordType.liftBoolTypes]
+      case _ ety heq =>
+        split at h₃
+        case _ =>
+          simp [ok, do_ok] at h₃
+          rcases h₃ with ⟨_, h₃₁, h₃₂⟩
+          subst h₃₂
+          simp [TypedExpr.liftBoolTypes]
+          simp [hasAttrInRecord] at h₃₁
+          split at h₃₁
+          · split at h₃₁ <;>
+          {
+            simp [ok] at h₃₁
+            rcases h₃₁ with ⟨h₃₁, _⟩
+            subst h₃₁
+            simp [CedarType.liftBoolTypes, BoolType.lift]
+            apply @TypedExpr.WellTyped.hasAttr_entity env ety
+            · exact typechecked_is_well_typed_after_lifting h₂ hᵢ
+            · simp [type_of_after_lifted_is_lifted, heq, CedarType.liftBoolTypes, RecordType.liftBoolTypes]
+          }
+          · simp [ok] at h₃₁
+            rcases h₃₁ with ⟨h₃₁, _⟩
+            subst h₃₁
+            simp [CedarType.liftBoolTypes, BoolType.lift]
+            apply @TypedExpr.WellTyped.hasAttr_entity env ety
+            · exact typechecked_is_well_typed_after_lifting h₂ hᵢ
+            · simp [type_of_after_lifted_is_lifted, heq, CedarType.liftBoolTypes, RecordType.liftBoolTypes]
+        case _ =>
+          split at h₃
+          · simp [ok] at h₃
+            rcases h₃ with ⟨h₃₁, h₃₂⟩
+            subst h₃₁
+            simp [TypedExpr.liftBoolTypes, CedarType.liftBoolTypes, BoolType.lift]
+            apply @TypedExpr.WellTyped.hasAttr_entity env ety
+            · exact typechecked_is_well_typed_after_lifting h₂ hᵢ
+            · simp [type_of_after_lifted_is_lifted, heq, CedarType.liftBoolTypes, RecordType.liftBoolTypes]
+          · simp [err] at h₃
+      case _ => simp [err] at h₃
+  case set ls =>
+    simp [typeOf] at h₃
+    simp [List.mapM₁_eq_mapM (λ x => justType (typeOf x c₁ env))] at h₃
+    sorry
   case record => sorry
-  case call => sorry
+  case call xfn args =>
+    sorry
+    /-
+    simp [typeOf] at h₃
+    simp [List.mapM₁_eq_mapM (λ x => justType (typeOf x c₁ env))] at h₃
+    generalize hᵢ : List.mapM (fun x => justType (typeOf x c₁ env)) args = res₁
+    cases res₁
+    case error => simp [hᵢ] at h₃
+    case ok ls =>
+      simp [hᵢ] at h₃
+      simp [List.mapM_ok_iff_forall₂] at hᵢ
+      simp [typeOfCall] at h₃
+      split at h₃ <;>
+      try simp [ok, do_ok] at h₃ <;>
+      rcases h₃ with ⟨_, h₃₁, h₃₂⟩ <;>
+      subst h₃₂ <;>
+      simp [TypedExpr.liftBoolTypes]
+      · apply TypedExpr.WellTyped.call
+        · simp [List.map₁_eq_map]
+          intro a h
+          rcases List.forall₂_implies_all_right hᵢ a h with ⟨_, _, h₄⟩
+          simp [justType, Except.map] at h₄
+          split at h₄
+          case _ => cases h₄
+          case _ e _ _ v heq =>
+            simp at h₄
+            have : v = (v.fst, v.snd) := by rfl
+            rw [this, h₄] at heq
+            exact typechecked_is_well_typed_after_lifting h₂ heq
+        · simp [typeOfConstructor] at h₃₁
+          split at h₃₁
+          · split at h₃₁
+            · rename_i heq
+              simp [ok] at h₃₁
+              rcases h₃₁ with ⟨h₃₁, _⟩
+              subst h₃₁
+              simp [CedarType.liftBoolTypes, List.map₁_eq_map]
+              cases hᵢ
+              · rename_i heq₁
+                cases heq₁
+                rename_i heq₂
+                simp [typeOf, typeOfLit, ok, justType, Except.map] at heq₂
+                subst heq₂
+                simp [TypedExpr.liftBoolTypes, CedarType.liftBoolTypes]
+                symm at heq
+                exact ExtFun.WellTyped.decimal heq
+            · simp [err] at h₃₁
+          · simp [err] at h₃₁
+      · sorry
+      · sorry
+      · sorry
+      · sorry
+      · sorry
+      · sorry
+      · sorry
+      · sorry
+      · sorry
+      · sorry
+      · sorry
+      · sorry
+      · sorry
+      · sorry
+      · sorry
+      · sorry
+      · sorry
+      · sorry
+      · sorry
+      · sorry
+      · sorry
+      · sorry
+  -/
 
 end Cedar.Thm
